

Assignment 10 Solutions

Basic Problems

$$\textcircled{1} \begin{bmatrix} 1 & -3 \\ 2 & -5 \end{bmatrix}^{-1} = \frac{1}{-5 - (-6)} \begin{bmatrix} -5 & 3 \\ -2 & 1 \end{bmatrix} = \begin{bmatrix} -5 & 3 \\ -2 & 1 \end{bmatrix}$$

$$\begin{aligned} \textcircled{2} & \begin{bmatrix} 1 & -3 & -2 & 1 & 0 & 0 \\ -3 & 10 & 8 & 0 & 1 & 0 \\ -2 & 5 & 3 & 0 & 0 & 1 \end{bmatrix} \sim \\ & \begin{bmatrix} 1 & -3 & -2 & 1 & 0 & 0 \\ 0 & 1 & 2 & 3 & 1 & 0 \\ 0 & -1 & -1 & 2 & 0 & 1 \end{bmatrix} \sim \\ & \begin{bmatrix} 1 & -3 & -2 & 1 & 0 & 0 \\ 0 & 1 & 2 & 3 & 1 & 0 \\ 0 & 0 & 1 & 5 & 1 & 1 \end{bmatrix} \sim \\ & \begin{bmatrix} 1 & -3 & 0 & 11 & 2 & 2 \\ 0 & 1 & 0 & -7 & -1 & -2 \\ 0 & 0 & 1 & 5 & 1 & 1 \end{bmatrix} \sim \\ & \begin{bmatrix} 1 & 0 & 0 & -10 & -1 & -4 \\ 0 & 1 & 0 & -7 & -1 & -2 \\ 0 & 0 & 1 & 5 & 1 & 1 \end{bmatrix} \end{aligned}$$

$$\begin{bmatrix} -10 & -1 & -4 \\ -7 & -1 & -2 \\ 5 & 1 & 1 \end{bmatrix}$$

③

$$\begin{aligned}\det(A - \lambda I) &= (2 - \lambda)(-5 - \lambda) + 12 \\&= -10 - 2\lambda + 5\lambda + \lambda^2 + 12 \\&= \lambda^2 + 3\lambda + 2 \\&= (\lambda + 2)(\lambda + 1)\end{aligned}$$

$$\lambda = -2, -1$$

$$A + I = \begin{bmatrix} 3 & -6 \\ 2 & -4 \end{bmatrix} \sim \begin{bmatrix} 1 & -2 \\ 0 & 0 \end{bmatrix} \quad \begin{bmatrix} 2 \\ 1 \end{bmatrix}$$

$$A + 2I = \begin{bmatrix} 4 & -6 \\ 2 & -3 \end{bmatrix} \sim \begin{bmatrix} 1 & -3/2 \\ 0 & 0 \end{bmatrix} \quad \begin{bmatrix} 3 \\ 2 \end{bmatrix}$$

$$P = \begin{bmatrix} 2 & 3 \\ 1 & 2 \end{bmatrix} \quad D = \begin{bmatrix} -1 & 0 \\ 0 & -2 \end{bmatrix}$$

$$\textcircled{4} \quad \begin{bmatrix} -2-\lambda & 0 & 0 \\ 2 & -1-\lambda & -1 \\ 6 & 4 & -5-\lambda \end{bmatrix} \sim \begin{bmatrix} -2-\lambda & 0 & 0 \\ 2(-5-\lambda) & (-1-\lambda)(-5-\lambda) & -(-5-\lambda) \\ 6 & 4 & -5-\lambda \end{bmatrix}$$

$$\begin{bmatrix} -2-\lambda & 0 & 0 \\ 2(-5-\lambda)+6 & (-1-\lambda)(-5-\lambda)+4 & 0 \\ 6 & 4 & -5-\lambda \end{bmatrix}$$

$$\det(A - \lambda I) = \frac{1}{-5-\lambda} (-2-\lambda) ((-1-\lambda)(-5-\lambda)+4) (-5-\lambda)$$

$$= (-2-\lambda)(5+\lambda+5\lambda+\lambda^2+4)$$

$$= -(\lambda+2)(\lambda^2+6\lambda+9)$$

$$= -(\lambda+2)(\lambda+3)^2$$

$$\lambda = -2, -3$$

$$A + 2I = \begin{bmatrix} 0 & 0 & 0 \\ 2 & 1 & -1 \\ 6 & 4 & -3 \end{bmatrix} \sim \begin{bmatrix} 2 & 1 & -1 \\ 0 & 1 & 0 \\ 0 & 0 & 0 \end{bmatrix} \sim$$

$$\begin{bmatrix} 1 & 0 & -\frac{1}{2} \\ 0 & 1 & 0 \\ 0 & 0 & 0 \end{bmatrix} \quad \begin{bmatrix} 1 \\ 0 \\ 2 \end{bmatrix}$$

$$A + 3I = \begin{bmatrix} 1 & 0 & 0 \\ 2 & 2 & -1 \\ 6 & 4 & -2 \end{bmatrix} \sim \begin{bmatrix} 1 & 0 & 0 \\ 0 & 2 & -1 \\ 0 & 4 & -2 \end{bmatrix}$$

$$\sim \begin{bmatrix} 1 & 0 & 0 \\ 0 & 1 & -\frac{1}{2} \\ 0 & 0 & 0 \end{bmatrix}$$

$$\begin{bmatrix} 0 \\ 1 \\ 2 \end{bmatrix}$$

Not diagonalizable. Does not have eigenbasis.

$$\textcircled{5} \quad \lambda(\lambda^2 - 2\lambda - 3) = \lambda(\lambda - 3)(\lambda + 1)$$

$$\lambda = 3, 0, -1$$

$$A - 3I = \begin{bmatrix} -4 & -3 & -6 \\ -8 & -9 & -12 \\ 4 & 3 & 6 \end{bmatrix} \sim \begin{bmatrix} -4 & -3 & -6 \\ 0 & -3 & -6 \\ 0 & 0 & 0 \end{bmatrix} \sim \begin{bmatrix} 1 & 0 & 0 \\ 0 & 1 & 2 \\ 0 & 0 & 0 \end{bmatrix}$$

$$\begin{bmatrix} 0 \\ -2 \\ 1 \end{bmatrix}$$

$$\begin{bmatrix} -1 & -3 & -6 \\ -8 & -6 & -18 \\ 4 & 3 & 9 \end{bmatrix} \sim \begin{bmatrix} 1 & 3 & 6 \\ 4^{-4} & 3^{-12} & 9^{-24} \\ 4 & 3 & 9 \end{bmatrix} \sim \begin{bmatrix} 1 & 3 & 6 \\ 0 & -9 & -15 \\ 0 & 0 & 0 \end{bmatrix}$$

$$\sim \begin{bmatrix} 1 & 3 & 6 \\ 0 & 3 & 5 \\ 0 & 0 & 0 \end{bmatrix} \sim \begin{bmatrix} 1 & 0 & 1 \\ 0 & 1 & 5/3 \\ 0 & 0 & 0 \end{bmatrix} \quad \begin{bmatrix} -3 \\ -5 \\ 3 \end{bmatrix}$$

$$A + I = \begin{bmatrix} 0 & -3 & -6 \\ -8 & -5 & -18 \\ 4 & 3 & 10 \end{bmatrix} \sim \begin{bmatrix} 4 & 3 & 10 \\ -8^{+8} & -5^{+6} & -18^{+20} \\ 0 & 1 & 2 \end{bmatrix} \sim \begin{bmatrix} 4 & 3 & 10 \\ 0 & 1 & 2 \\ 0 & 0 & 0 \end{bmatrix}$$

$$\sim \begin{bmatrix} 4 & 0 & 4 \\ 0 & 1 & 2 \\ 0 & 0 & 0 \end{bmatrix} \sim \begin{bmatrix} 1 & 0 & 1 \\ 0 & 1 & 2 \\ 0 & 0 & 0 \end{bmatrix} \quad \begin{bmatrix} -1 \\ -2 \\ 1 \end{bmatrix}$$

$$P = \begin{bmatrix} 0 & -3 & -1 \\ -2 & -5 & -2 \\ 1 & 3 & 1 \end{bmatrix}$$

$$D = \begin{bmatrix} 3 & 0 & 0 \\ 0 & 0 & 0 \\ 0 & 0 & -1 \end{bmatrix}$$

$$\textcircled{6} \quad a. \quad \|\vec{v}_1\| = \sqrt{49+9} = \sqrt{58} \quad \|\vec{v}_2\| = \sqrt{1+25} = \sqrt{26}$$

$$b. \quad \langle \vec{v}_1, \vec{v}_2 \rangle = 7(-1) + 3(5) = -7 + 15 = 8$$

$$\cos^{-1} \left(\frac{8}{\sqrt{58} \cdot \sqrt{26}} \right) \approx 1.36 \text{ rad}$$

$$c. \quad \|\vec{v}_1 - \vec{v}_2\| = \left\| \begin{bmatrix} 8 \\ -2 \end{bmatrix} \right\| = \sqrt{64+4} = \sqrt{68}$$

$$d. \quad \frac{\vec{v}_1}{\|\vec{v}_1\|} = \frac{1}{\sqrt{58}} \begin{bmatrix} 7 \\ 3 \end{bmatrix} \quad \frac{\vec{v}_2}{\|\vec{v}_2\|} = \frac{1}{\sqrt{26}} \begin{bmatrix} -1 \\ 5 \end{bmatrix}$$

$$\textcircled{7} \quad a. \quad \|\vec{v}_1\| = \sqrt{4+16+25} = \sqrt{45} \quad \|\vec{v}_2\| = \sqrt{4+4+4} = \sqrt{12}$$

$$b. \quad \langle \vec{v}_1, \vec{v}_2 \rangle = -2(2) + 4(2) + (-5)(-2) = -4 + 8 + 10 = 14$$

$$\cos^{-1} \left(\frac{14}{\sqrt{45} \sqrt{12}} \right) \approx 0.92 \text{ rad}$$

$$c. \quad \|\vec{v}_1 - \vec{v}_2\| = \left\| \begin{bmatrix} -4 \\ 2 \\ -3 \end{bmatrix} \right\| = \sqrt{16+4+9} = \sqrt{29}$$

$$d. \quad \frac{\vec{v}_1}{\|\vec{v}_1\|} = \frac{1}{\sqrt{45}} \begin{bmatrix} -2 \\ 4 \\ -5 \end{bmatrix} \quad \frac{\vec{v}_2}{\|\vec{v}_2\|} = \frac{1}{\sqrt{12}} \begin{bmatrix} 2 \\ 2 \\ -2 \end{bmatrix} = \begin{bmatrix} \frac{\sqrt{3}}{3} \\ \frac{\sqrt{3}}{3} \\ -\frac{\sqrt{3}}{3} \end{bmatrix}$$

True / False

1. True

2. False $\begin{bmatrix} 0 & 0 \\ 0 & 0 \end{bmatrix}$

3. True

4. False $\begin{bmatrix} 1 & 0 \\ 0 & 2 \end{bmatrix}$ & $\begin{bmatrix} -1 & 1 \\ -6 & 4 \end{bmatrix}$

5. False $\begin{bmatrix} 1 & 0 \\ 0 & 1 \end{bmatrix}$

6. False $\begin{bmatrix} 1 & 0 \\ 0 & 0 \end{bmatrix}$

7. False $\begin{bmatrix} 1 & 0 \\ 0 & 2 \end{bmatrix} = \begin{bmatrix} 0 & 1 \\ 1 & 0 \end{bmatrix} \begin{bmatrix} 2 & 0 \\ 0 & 1 \end{bmatrix} \begin{bmatrix} 0 & 1 \\ 1 & 0 \end{bmatrix}$

8. True

9. False $\begin{bmatrix} 1 & 0 \\ 1 & 0 \end{bmatrix}$ $\begin{bmatrix} 1 \\ 1 \end{bmatrix} \in \text{Col}(A)$
 $\begin{bmatrix} 0 \\ 1 \end{bmatrix} \in \text{Nul}(A)$

More Difficult Problems

$$\textcircled{1} \quad -\lambda^3 + 5\lambda^2 - 6\lambda = -\lambda(\lambda^2 - 5\lambda + 6) \\ = -\lambda(\lambda - 3)(\lambda - 2)$$

$$\lambda = 3, 2, 0$$

$$A - 3I = \begin{bmatrix} -3 & 3 & -3 \\ -2 & 3 & -4 \\ -2 & 3 & -4 \end{bmatrix} \sim \begin{bmatrix} 1 & -1 & 1 \\ 2 & -3 & 4 \\ 0 & 0 & 0 \end{bmatrix} \sim \begin{bmatrix} 1 & -1 & 1 \\ 0 & 1 & -2 \\ 0 & 0 & 0 \end{bmatrix}$$

$$\sim \begin{bmatrix} 1 & 0 & -1 \\ 0 & 1 & -2 \\ 0 & 0 & 0 \end{bmatrix} \quad \text{Nul}(A - 3I) = \text{span} \left\{ \begin{bmatrix} 1 \\ 2 \\ 1 \end{bmatrix} \right\}$$

$$A - 2I = \begin{bmatrix} -2 & 3 & -3 \\ -2 & 4 & -4 \\ -2 & 3 & -3 \end{bmatrix} \sim \begin{bmatrix} 1 & -2 & 2 \\ -2 & 4 & -4 \\ 0 & 0 & 0 \end{bmatrix} \sim \begin{bmatrix} 1 & -2 & 2 \\ 0 & -1 & 1 \\ 0 & 0 & 0 \end{bmatrix}$$

$$\begin{bmatrix} 1 & 0 & 0 \\ 0 & 1 & -1 \\ 0 & 0 & 0 \end{bmatrix} \quad \text{Nul}(A - 2I) = \left\{ \begin{bmatrix} 0 \\ 1 \\ 1 \end{bmatrix} \right\}$$

$$A = \begin{bmatrix} 0 & 3 & -3 \\ -2 & 6 & -4 \\ -2 & 3 & -1 \end{bmatrix} \sim \begin{bmatrix} 1 & -3 & 2 \\ -2 & 3 & -6 \\ 0 & 1 & -1 \end{bmatrix} \sim \begin{bmatrix} 1 & -3 & 2 \\ 0 & -3 & 3 \\ 0 & 1 & -1 \end{bmatrix}$$

$$\sim \begin{bmatrix} 1 & -3 & 2 \\ 0 & 1 & -1 \\ 0 & 0 & 0 \end{bmatrix} \sim \begin{bmatrix} 1 & 0 & -1 \\ 0 & 1 & -1 \\ 0 & 0 & 0 \end{bmatrix} \quad \text{Nul}(A) = \left\{ \begin{bmatrix} 1 \\ 1 \\ 1 \end{bmatrix} \right\}$$

2.

$$\textcircled{a} \quad \lambda = 0 \Rightarrow \dim(\text{Nul}(A)) \geq 1$$

$$\dim(\text{Nul}(A)) \leq 1 \quad \text{since deg. in char. poly} = 1$$

$$\Rightarrow \dim(\text{Nul}(A)) = 1 \quad \text{and}$$

$$\text{rank}(A) + \dim(\text{Nul}(A)) = 5 \Rightarrow \dim(\text{Nul}(A)) = 4$$

$$\textcircled{b} \quad \lambda = 2, 0, -1$$

$$\text{rank}(A - 2I) + \dim(\text{Nul}(A - 2I)) = 5$$

$$\text{rank}(A - 2I) = 3$$

\Downarrow

$$\dim(\text{Nul}(A - 2I)) = 2$$

$$\text{rank}(A + I) + \dim(\text{Nul}(A + I)) = 5$$

$$\text{rank}(A + I) = 3$$

\Downarrow

$$\dim(\text{Nul}(A + I)) = 2$$

$\Rightarrow A$ has an eigenbasis $\Rightarrow A$ is diagonalizable

$$\textcircled{3} \quad P = [\vec{p}_1 \quad \dots \quad \vec{p}_n] \quad D = [d_1 \vec{e}_1 \quad \dots \quad d_n \vec{e}_n]$$

$$AP = [A\vec{p}_1 \quad \dots \quad A\vec{p}_n]$$

$$PD = [P(d_1 \vec{e}_1) \quad \dots \quad P(d_n \vec{e}_n)] = [d_1 P\vec{e}_1 \quad \dots \quad d_n P\vec{e}_n] \\ = [d_1 \vec{p}_1 \quad \dots \quad d_n \vec{p}_n]$$

$$AP = PD \Rightarrow A\vec{p}_1 = d_1 \vec{p}_1 \quad \text{and} \dots \quad \text{and} \quad A\vec{p}_n = d_n \vec{p}_n$$

eigenvalues
eigenvector
if $\vec{p}_i \neq \vec{0}$

$$\textcircled{4} \quad A \begin{bmatrix} 1 & -2 & -1 & 3 \\ 3 & -6 & -7 & 2 \end{bmatrix} \begin{bmatrix} x_1 \\ x_2 \\ x_3 \\ x_4 \end{bmatrix} = \begin{bmatrix} 0 \\ 0 \end{bmatrix}$$

-3 +6 +3 -9

$$\begin{bmatrix} 1 & -2 & -1 & 3 \\ 0 & 0 & 1 & -7 \end{bmatrix} \sim \begin{bmatrix} 1 & -2 & 0 & -4 \\ 0 & 0 & 1 & -7 \end{bmatrix}$$

$$x_1 = 2x_2 + 4x_4$$

x_2 is free

$$x_3 = 7x_4$$

x_4 is free

$$\dim(\text{Nul}(A)) = 2$$

⑤

$$\begin{aligned}\cos^{-1}\left(\frac{\langle a\vec{u}, b\vec{v} \rangle}{\|a\vec{u}\| \cdot \|b\vec{v}\|}\right) &= \cos^{-1}\left(\frac{\cancel{a}\cancel{b}\langle u, v \rangle}{\cancel{a}\|\vec{u}\| \cdot \cancel{b}\|\vec{v}\|}\right) \\ &= \cos^{-1}\left(\frac{\langle u, v \rangle}{\|\vec{u}\| \cdot \|\vec{v}\|}\right)\end{aligned}$$